\documentclass[a4paper, fontsize=10bp]{article} % преамбула документа
\usepackage{scrextend}
\usepackage[left=2.0cm, right=1.5cm, top=2.0cm,
bottom=2.0cm]{geometry}
\usepackage[utf8]{inputenc}
\usepackage[T2A]{fontenc}
\usepackage{hyperref}
\usepackage[english, russian]{babel}
\usepackage{amsmath,amsfonts,amssymb}
\usepackage{graphicx}
\usepackage{setspace}
\usepackage{fontsize}



\begin{document} % тело документа

\begin{align*}
    \lim  _{x \to a} \frac{a^x - x^a} {\sqrt[3]{ax^2} -acos(x-a)} = 
\end{align*}

\section*{4.}
\begin{align*}
    &\lim_{x \to a} \frac{\log(x + \sqrt{x^2 - 4}) - \log(a + \sqrt{a^2 - 4})}{x - a}  = \lim_{x \to a} \left[\frac{\log \left( \frac{x + \sqrt{x^2 - 4}}{a + \sqrt{a^2 - 4}} \right)} {x-a} \right.\\
    = &\left.\frac{\log \left( 1 + \frac{x + \sqrt{x^2 - 4} - a - \sqrt{a^2 - 4}}{a+\sqrt{a^2 - 4}} \right)}{x-a} \right. = \left. \frac{\log \left(   1 + \frac{x - a}{a + \sqrt{a^2 - 4}} + \frac{x^2 - a^2}{\left(a + \sqrt{a^2 - 4} \right) \left( \sqrt{a^2 - 4} + \sqrt{a^2 + 4}\right)} \right)}{x-a} = \right. \\   
    =&\left.\frac{\frac{x-a}{\cdots} + \frac{x-a}{\cdots}(x + a) + 0(x-a)}{x-a} = \frac{1}{a + \sqrt{a^2 - 4}}\left(1 + \frac{2a}{2\sqrt{a^2 -4}}\right)\right]\\
\end{align*}

\begin{align*}
    &\left(\log(x+\sqrt{x^2-4})\right)' = \frac{1}{x+\sqrt{x^2-4}}\left(1 + \frac{2x}{2\sqrt{x^2-4}}\right)
\end{align*}


\end{document}